pcuic/theories/PCUICTypedAst.v
@@ -9,7 +9,7 @@ Require Vector Fin.
 Section Branch.
   Context {term : nat -> Type}.
   (* Parameterized by term types as they are not yet defined. *)
-  Record branch := mkbranch {
+  Record branch := mk_branch {
     bcontext : list (context_decl term); 
     (* Context of binders of the branch, including lets. *)
     bbody : term; (* The branch body *) }.
@@ -19,7 +19,7 @@ Arguments branch : clear implicits.
 
 (* Defined here since BasicAst does not have access to universe instances.
   Parameterized by term types as they are not yet defined. *)
-Record predicate {term} := mkpredicate {
+Record predicate {term} := mk_predicate {
   pparams : list term; (* The parameters *)
   puinst : Instance.t; (* The universe instance *)
   pcontext : list (context_decl term); (* The predicate context, 
@@ -27,7 +27,7 @@ Record predicate {term} := mkpredicate {
   preturn : term; (* The return type *) }.
   Derive NoConfusion for predicate.
 Arguments predicate : clear implicits.
-Arguments mkpredicate {_}.
+Arguments mk_predicate {_}.
   *)
 
 Inductive context (P : nat -> Type) : nat -> Type :=
